\documentclass[journel,11pt,two column]{IEEEtran}
\usepackage{amsmath, amssymb,amsfonts}
\usepackage{enumitem}
\usepackage{tfrupee}
\vspace{3cm}
  
  
\title{AI1110 Assignment I (ICSE Class 10 2019)}
\author{sumeeth kumar(ai21btech11008)}
\date{april 2022}
% make the title area


\begin{document}
\maketitle
\textbf{Question 2(b):}
 \textbf{ prove that}\\
  ${(\csc \theta - \sin \theta)(\sec \theta -\cos \theta)(\tan \theta +\cot \theta)}$=1 \\  
 \textbf{solution:}   Given that in the equation, RHS=1.\\ 
 we thave to show LHS = RHS , i.e 1.\\  
 \textbf{LHS} $=(\csc \theta - \sin \theta)(\sec \theta -\cos \theta)(\tan \theta +\cot \theta)$\\
 we know that,
 \begin{align}
  \csc\theta = \frac{1}{
  \sin \theta}\\[8pt]
  \sec\theta = \frac{1}{\cos \theta}\\[8pt]
  \tan\theta = \frac{\sin\theta}{\cos\theta}=\frac{1}{\tan \theta}\\[8pt]
  \sin^2\theta+\cos^2\theta=1
 \end{align} 
 
 \vspace{0.1cm}
 
 \begin{center}
  from eqns 1,2, 3,4\\[8pt]
 \end{center}
\begin{align*}
 &{LHS=\left(\frac{1}{\sin\theta}-\sin\theta    \right)\left(\frac{1}{\cos\theta}-\cos\theta \right)\left(\frac{\sin\theta}{\cos\theta}+\frac{\cos\theta}{\sin\theta}\right)}\\[8pt]  
 &{ LHS=\left(\frac{1-\sin^2\theta}{\sin\theta}\right)\left(\frac{1-\cos^2\theta}{\cos\theta}\right)\left(\frac{\sin^2\theta+\cos^2\theta}{\sin\theta \cos\theta}\right)}\\[8pt]
 &{LHS=\left(\frac{\cos^2\theta}{\sin\theta}\right)\left(\frac{\sin^2\theta}{\cos\theta}\right)\left(\frac{1}{\sin\theta \cos\theta}\right)}\\[8pt]
 &{LHS=\left(\frac{\sin^2\theta \cos^2\theta}{\sin^2\theta \cos^2\theta}\right)}\\[8pt]
 &{LHS=1=RHS}
\end{align*}
\begin{center}
\fbox{$\therefore {LHS=RHS}$}\\ 
[8pt]
\end{center}

 Hence proved that ${(\csc \theta - \sin \theta)(\sec \theta -\cos \theta)(\tan \theta +\cot \theta)}$=1 \\  
 
\end{document}
